Added substitution based evaluator

simple/subst.v
@@ -23,6 +23,7 @@ Definition import_exp {α β} (x:α↪β) : exp α -> exp β :=
  rename (import x).
 
 Reserved Notation "[ θ ] T" (at level 90).
+
 Fixpoint app_subst {α β} (θ:name α -> exp β) (M:exp α) : exp β :=
 match M with
 | var n => θ n
@@ -46,11 +47,11 @@ econstructor.
 set (next_link γ0).
 eapply IHof.
 intros.
-unfold compose.
+unfold compose at 2 4.
 case (export x x0); simpl; intros.
-erewrite export_import_inv.
+unfold compose. erewrite export_import_inv.
 simpl. eauto.
-erewrite export_self.
+unfold compose. erewrite export_self.
 reflexivity.
 Qed.
 
@@ -66,18 +67,64 @@ set (next_link γ0).
 econstructor.
 eapply IHof.
 intro.
-unfold import_exp.
-unfold compose.
-remember (export x x0).
-destruct s.
-simpl.
-specialize (H0 n).
-eapply rename_lemma.
-eassumption.
-intros. erewrite export_import_inv.
+unfold compose at 2 4.
+case (export x x0); intros; simpl.
+eapply rename_lemma; eauto.
+intros. unfold compose. erewrite export_import_inv.
 reflexivity.
 econstructor.
-erewrite export_self.
+unfold compose. erewrite export_self.
 reflexivity.
 Qed.
 
+(* Single substitution practically requires simultaneous?*)
+Definition single_subst {γ γ'} (x:γ↪γ') (M:exp γ') (N:exp γ) := [@var γ,,(x,N)] M. 
+
+Lemma single_subst_lemma : forall {γ γ'} (x:γ↪γ') M N U T (Γ:tp_ctx γ),
+  Γ,,(x,U) ⊢ M ⇐ T ->
+  Γ ⊢ N ⇐ U 
+(*====================*) ->
+  Γ ⊢ single_subst x M N ⇐ T.
+intros.
+eapply subst_lemma.
+eexact H.
+intro. unfold compose.
+case (export x x0); intros; simpl; eauto.
+Qed.
+
+Inductive val : exp ∅ -> Prop :=
+| tt_val : val tt
+| lam_val : forall {γ} {x:∅↪γ} M T, val (lam x T M)
+| inl_val : forall M T, val M -> val (inl T M)
+| inr_val : forall M T, val M -> val (inr T M).
+
+Reserved Notation "M ⇓ V" (at level 90).
+Inductive eval : exp ∅ -> exp ∅ -> Prop :=
+| eval_val : forall V, val V -> eval V V
+| eval_app : forall M {γ} T (x:∅↪γ) (M':exp γ) N V1 V2 ,
+     M ⇓ (lam x T M') ->
+     N ⇓ V1 ->
+     (single_subst x M' V1) ⇓ V2 ->
+     (app M N) ⇓ V2 
+| eval_inl : forall M T V,
+     M ⇓ V ->
+     (inl T M) ⇓ (inl T V)
+| eval_inr : forall M T V,
+     M ⇓ V ->
+     (inr T M) ⇓ (inr T V)
+where "M ⇓ V" := (eval M V).
+
+Hint Constructors eval.
+Theorem subject_reduction M V : M ⇓ V -> forall T, · ⊢ M ⇐ T -> · ⊢ V ⇐ T.
+induction 1; intros; eauto.
+nice_inversion H2.
+eapply IHeval3.
+eapply single_subst_lemma.
+apply IHeval1 in H5.
+nice_inversion H5.
+eassumption.
+apply IHeval2.
+assumption.
+nice_inversion H0. eauto.
+nice_inversion H0. eauto.
+Qed.
